

GPEC field line tracing maths

Some definitions:

- η = machine poloidal angle
- ϕ = machine toroidal angle
- r = machine minor radius
- R = machine major radius
- θ = magnetic poloidal angle
- ζ = magnetic toroidal angle
- subscript N : ‘normalized’
- $bf\%f = RB_\phi = F(\psi)$ (see Ideal MHD equ 6.11)
- $\psi_0 = \psi$ on axis, $\psi_a = \psi$ at separatrix

$$\begin{aligned} q &= \frac{F(\psi)}{2\pi} \oint \frac{dl_p}{R^2 B_p} \\ &= \frac{1}{2\pi} \oint \frac{dl_p B_\phi}{R B_p} \end{aligned}$$

y_out spline:

$y_out(0) = \eta$ machine poloidal angle ($\mathbf{F}_p \Leftrightarrow \mathbf{F}_\eta$)

$y(1)$

$$\begin{aligned} \frac{dy(1)}{d\eta} &= \frac{r}{B_z \cos(\eta) - B_R \sin(\eta)} = \frac{r}{B_\eta} \\ \Rightarrow dy(1) &= \frac{r d\eta}{B_\eta} = \frac{dl_p}{B_\eta} \\ \Rightarrow y(1) &= \int \frac{dl_\eta}{B_\eta} \\ \Rightarrow y(1)|_{2\pi} &= \oint \frac{dl_\eta}{B_\eta} =? \frac{dV}{d\psi} \frac{1}{2\pi} \text{ (see Freidberg Ideal MHD equ 6.22, } dl_p \text{ is poloidal arc length)} \end{aligned}$$

y(2)

$$\begin{aligned}
\frac{dr}{dl_\eta} &= \frac{B_r}{B_\eta} \\
\Rightarrow \frac{dr}{rd\eta} &= \frac{B_r}{B_\eta} \\
\Rightarrow \frac{dr}{d\eta} &= \frac{B_r}{B_\eta} r \\
\frac{dy(2)}{d\eta} &= \frac{dy(1)}{d\eta} [B_R \cos(\eta) + B_Z \sin(\eta)] = \frac{B_r}{B_\eta} r \\
\Rightarrow y(2) &= r
\end{aligned}$$

y(3)

$$\begin{aligned}
\frac{dy(3)}{d\eta} &= \frac{dy(1)/d\eta}{R^2} = \frac{r}{R^2 B_\eta} \\
\Rightarrow y(3) &= \int \frac{dl_\eta}{R^2 B_\eta} \\
\Rightarrow y(3)|_{2\pi} &= 2\pi \frac{q(\psi)}{F(\psi)} \quad (\text{see Ideal MHD equ 6.35})
\end{aligned}$$

y(4) Should be unnormalised magnetic poloidal angle θ

$$\begin{aligned}
\frac{dy(4)}{d\eta} &= \frac{dy(1)}{d\eta} \left[\frac{B_p^{\alpha_p} (|B|)^{\alpha_B}}{R^{\alpha_R}} \right] \\
&= \frac{r}{B_\eta} \left[\frac{B_p^{\alpha_p} (|B|)^{\alpha_B}}{R^{\alpha_R}} \right] \\
&\propto \frac{r}{B_\eta} (B \cdot \nabla \theta) \\
&= \frac{r}{B_\eta} (B_\theta) \\
\Rightarrow \frac{dy(4)}{rd\eta} &= \frac{dy(4)}{dl_\eta} = \frac{B_\theta}{B_\eta} \\
\Rightarrow y(4) &= \theta
\end{aligned}$$

ff spline:

ff%xs Normalised magnetic poloidal angle θ_N

$$\text{ff}\%xs = \frac{y(4)}{y(4)|_{\eta=2\pi}} = \frac{\theta(\eta)}{\theta(\eta = 2\pi)}$$

$$\text{ff}\%f(1) = r^2$$

$$\text{ff}\%f(2) = \text{normalised } \eta - \text{normalised } \theta$$

$$= \frac{\eta}{2\pi} - \frac{y(4)|_{\eta}}{y(4)|_{\eta=2\pi}}$$

$$= \frac{\eta}{2\pi} - \frac{\theta(\eta)}{\theta(\eta=2\pi)}$$

$$\text{ff}\%f(3) = \phi(\eta) - \zeta(\eta)$$

$$\begin{aligned} ff\%f(3) &= F \left(\int^{\eta} \frac{r}{R^2 B_{\eta}} d\eta - \theta_N(\eta) \oint \frac{r}{R^2 B_{\eta}} d\eta \right) \\ &= F \left(\int^{\eta} \frac{r}{R^2 B_{\eta}} d\eta - \theta_N(\eta) \oint \frac{r}{R^2 B_{\eta}} d\eta \right) \\ &= F \int^{\eta} \frac{r}{R^2 B_{\eta}} d\eta - \theta_N(\eta) F \oint \frac{r}{R^2 B_{\eta}} d\eta \\ &= F \int^{\eta} \frac{r}{R^2 B_{\eta}} d\eta - \theta_N(\eta) [F \oint \frac{r}{R^2 B_{\eta}} d\eta] \\ &= \int^{\eta} \frac{r}{R} \frac{B_{\phi}}{B_{\eta}} d\eta - \theta_N(\eta) \left[\oint \frac{r}{R} \frac{B_{\phi}}{B_{\eta}} d\eta \right] \\ &= \int^{l_{\eta}} \frac{1}{R} \frac{B_{\phi}}{B_{\eta}} dl_{\eta} - \theta_N(\eta) \left[\oint \frac{1}{R} \frac{B_{\phi}}{B_{\eta}} dl_{\eta} \right] \\ &= \int^{l_{\eta}} \frac{1}{R} \frac{dl_{\phi}}{dl_{\eta}} dl_{\eta} - \theta_N(\eta) \left[\oint \frac{1}{R} \frac{dl_{\phi}}{dl_{\eta}} dl_{\eta} \right] \\ &= \int^{l_{\phi}(\eta)} \frac{1}{R} dl_{\phi} - \theta_N(\eta) \left[\oint \frac{1}{R} dl_{\phi} \right] \\ &= \int^{\phi(\eta)} \frac{1}{R} R d\phi - \theta_N(\eta) \left[\oint \frac{1}{R} R d\phi \right] \\ &= \int^{\phi(\eta)} d\phi - \theta_N(\eta) \left[\oint d\phi \right] \\ &= \phi(\eta) - \theta_N(\eta) \phi(\eta = 2\pi) \\ &= \phi(\eta) - \zeta(\eta) \end{aligned}$$

Note $\theta_N(\eta)$ varies from 0 to 1 as η increases. $\phi(\eta = 2\pi)$ is to ensure normalisation.

$$\text{ff}\%f(4) = \text{normalised } \frac{dV}{d\psi} - \theta_N(\eta)$$

$$= \frac{dV}{d\psi}(\eta) / \left[\frac{dV}{d\psi}(\eta = 2\pi) \right] - \theta_N(\eta)$$

rzphi spline:

rzphi(i) = ff%f(i) for i = 1,2,3.

rzphi(4) = 'jacobian'

[in this section, J is the jacobian, not current]

$$\begin{aligned}
d\mathbf{r} &= RdRdZd\phi \\
&= Jd\psi d\theta d\zeta \\
V &= \int d\mathbf{r} \\
&= \int Jd\psi d\theta d\zeta \\
&= \oint d\zeta \int_{\psi_o}^{\psi} d\psi \oint J(\theta, \psi) \\
&= \int_0^1 d\zeta \int_{\psi_o}^{\psi} d\psi \oint d\theta J(\theta, \psi) \\
&= \int_{\psi_o}^{\psi} d\psi \oint d\theta J(\theta, \psi) \\
\frac{dV}{d\psi} &= \oint d\theta J(\theta, \psi) \\
\Rightarrow J(\theta, \psi) &= \frac{d}{d\theta} \frac{dV}{d\psi}
\end{aligned}$$

$$\begin{aligned}
\text{rzphi}(4)(\theta) &= \left(1 + \frac{d}{d\theta_N} f f \% f(4)\right) \times y(1)|_{\theta_N=1} \times 2\pi \times psio \\
&= \left(1 + \frac{d}{d\theta_N} \left[\frac{\frac{dV}{d\psi}(\theta_N)}{\frac{dV}{d\psi}(\theta_N=1)} - \theta_N \right]\right) \times \frac{dV}{d\psi}(\theta_N=1) \times (\psi_a - \psi_0) \\
&= \left(1 + \frac{1}{\frac{dV}{d\psi}(\theta_N=1)} \frac{d}{d\theta_N} \frac{dV}{d\psi}(\theta_N) - \frac{d}{d\theta_N} \theta_N\right) \times \frac{dV}{d\psi}(\theta_N=1) \times (\psi_a - \psi_0) \\
&= \left(1 + \frac{1}{\frac{dV}{d\psi}(\theta_N=1)} \frac{d}{d\theta_N} \frac{dV}{d\psi}(\theta_N) - 1\right) \times \frac{dV}{d\psi}(\theta_N=1) \times (\psi_a - \psi_0) \\
&= \left(\frac{d}{d\theta_N} \frac{dV}{d\psi}(\theta_N)\right) \times (\psi_a - \psi_0) \\
&= J \times (\psi_a - \psi_0) \text{ (this is the Jacobian with real units of } \psi.)
\end{aligned}$$